theories/unscoped.v
@@ -58,22 +58,6 @@ Class Ren5 (X1 X2 X3 X4 X5 : Type) (Y Z : Type) :=
 Declare Scope fscope. 
 Declare Scope subst_scope.
 
-Notation "s ⟨ xi1 ⟩" := (ren1 xi1 s) (at level 7, left associativity, format "s  ⟨ xi1 ⟩") : subst_scope.
-
-Notation "s ⟨ xi1 ; xi2 ⟩" := (ren2 xi1 xi2 s) (at level 7, left associativity, format "s  ⟨ xi1 ; xi2 ⟩") : subst_scope.
-
-Notation "s ⟨ xi1 ; xi2 ; xi3 ⟩" := (ren3 xi1 xi2 xi3 s) (at level 7, left associativity, format "s  ⟨ xi1 ; xi2 ; xi3 ⟩") : subst_scope.
-
-Notation "s ⟨ xi1 ; xi2 ; xi3 ; xi4 ⟩" := (ren4  xi1 xi2 xi3 xi4 s) (at level 7, left associativity, format "s  ⟨ xi1 ; xi2 ; xi3 ; xi4 ⟩") : subst_scope.
-
-Notation "s ⟨ xi1 ; xi2 ; xi3 ; xi4 ; xi5 ⟩" := (ren5  xi1 xi2 xi3 xi4 xi5 s) (at level 7, left associativity, format "s  ⟨ xi1 ; xi2 ; xi3 ; xi4 ; xi5 ⟩") : subst_scope.
-
-Notation "⟨ xi ⟩" := (ren1 xi) (at level 1, left associativity, format "⟨ xi ⟩") : fscope.
-
-Notation "⟨ xi1 ; xi2 ⟩" := (ren2 xi1 xi2) (at level 1, left associativity, format "⟨ xi1 ; xi2 ⟩") : fscope.
-
-
-
 (** *** Type Classes for Substiution *)
 
 Class Subst1 (X1 : Type) (Y Z: Type) :=
@@ -90,11 +74,6 @@ Class Subst4 (X1 X2 X3 X4: Type) (Y Z: Type) :=
 
 Class Subst5 (X1 X2 X3 X4 X5 : Type) (Y Z: Type) :=
   subst5 : X1 -> X2 -> X3 -> X4 -> X5  -> Y  -> Z.
-
-Notation "s [ sigma ]" := (subst1 sigma s) (at level 7, left associativity, format "s '/' [ sigma ]") : subst_scope.
-
-Notation "s [ sigma ; tau ]" := (subst2 sigma tau s) (at level 7, left associativity, format "s '/' [ sigma ; '/'  tau ]") : subst_scope.
-
 
 (** *** Type Class for Variables *)
 
